bst start

data-structures/Binary_tree.v
@@ -1,7 +1,62 @@
 
+Require Import Coq.Strings.String.
+
+Module Binary_search_tree.
+
+Notation "∀ A , B" := (forall A , B) (at level 200).
+
+Notation "∃ A , B" := (exists A , B) (at level 200).
 
 
-Module Binary_tree.
+Inductive tree (K V: Type) : Type := 
+| Leaf
+| Node (l: tree K V) (key: K) (val: V) (r: tree K V).
+
+Arguments Leaf {K V}.
+Arguments Node {K V}.
+
+Definition cmp {K: Type} := K -> K -> bool.
 
 
-End Binary_tree.
+Fixpoint lookup {K V : Type} (x : K) (t : tree K V) (less: @cmp K) : 
+        option V :=
+  match t with
+  | Leaf => None
+  | Node l y v r => if (less x y) then lookup x l less
+                 else if (less y x) then lookup x r less
+                     else Some v
+  end.
+
+Fixpoint insert {K V : Type} (x : K) (v : V) (t : tree K V) (less: @cmp K) : tree K V :=
+  match t with
+  | Leaf => Node Leaf x v Leaf
+  | Node l y v' r => if (less x y) then Node (insert x v l less) y v' r
+                 else if (less y x) then Node l y v' (insert x v r less)
+                      else Node l x v r
+  end.
+
+
+Module Tests.
+Open Scope string_scope.
+
+Definition test_tree := Node (Node Leaf 2 "two" (Node Leaf 3 "three" Leaf)) 4 "four" Leaf.
+
+Example tree_test1 :
+     insert 3 "three"
+     (insert 2 "two" 
+     (insert 4 "four" Leaf Nat.ltb) 
+     Nat.ltb) Nat.ltb = test_tree.
+  Proof. simpl. reflexivity. Qed.
+
+Example tree_test2 :
+     lookup 3 test_tree Nat.ltb = Some "three".
+  Proof. simpl. reflexivity. Qed.
+
+Example tree_test3 :
+lookup 5 test_tree Nat.ltb = None.
+Proof. simpl. reflexivity. Qed.
+End Tests.
+
+
+
+End Binary_search_tree.
